restructure

src/defs.lean
@@ -91,3 +91,286 @@ inductive or_instance (Γ : list nnf) : list nnf → list nnf → Type
 
 def left_prcp : Π {Γ₁ Γ₂ Δ : list nnf} (i : or_instance Δ Γ₁ Γ₂), nnf 
 | Γ₁ Γ₂ Δ (@or_instance.cons _ φ ψ _) := φ
+
+@[simp] def sub_nnf : nnf → list nnf
+| (var n)    := [var n]
+| (neg n)    := [neg n]
+| (and φ ψ)  := and φ ψ :: (sub_nnf φ ++ sub_nnf ψ)
+| (or φ ψ)   := or φ ψ :: (sub_nnf φ ++ sub_nnf ψ)
+| (box φ)    := box φ :: sub_nnf φ
+| (dia φ)    := dia φ :: sub_nnf φ
+
+theorem mem_sub_nnf_self : Π φ : nnf, φ ∈ sub_nnf φ :=
+begin intro φ, cases φ,  all_goals {simp} end 
+
+theorem mem_sub_nnf_and {φ ψ : nnf} : Π γ : nnf, and φ ψ ∈ sub_nnf γ → φ ∈ sub_nnf γ ∧ ψ ∈ sub_nnf γ
+| (var n) h   := begin simp at h, contradiction end
+| (neg n) h   := begin simp at h, contradiction end 
+| (and φ₁ ψ₁) h := 
+begin 
+simp only [sub_nnf] at h, 
+cases h, 
+{injection h with eq₁ eq₂, 
+ rw eq₁, rw eq₂, 
+ simp only [sub_nnf], 
+ split, 
+ {simp, right, left, apply mem_sub_nnf_self}, 
+ {simp, right, right, apply mem_sub_nnf_self}},
+{have := (@list.mem_append _ _ _ _).1 h,  
+ cases this,
+ {split,
+  {simp, right, left, apply (mem_sub_nnf_and _ _).1, exact this},
+  {simp, right, left, apply (mem_sub_nnf_and _ _).2, exact this}},
+ {split, 
+  {simp, right, right, apply (mem_sub_nnf_and _ _).1, exact this},
+  {simp, right, right, apply (mem_sub_nnf_and _ _).2, exact this}}}
+end
+| (or φ₁ ψ₁) h  := 
+begin 
+simp at h,
+cases h,
+ {split,
+  {simp, right, left, apply (mem_sub_nnf_and _ _).1, exact h},
+  {simp, right, left, apply (mem_sub_nnf_and _ _).2, exact h}},
+ {split, 
+  {simp, right, right, apply (mem_sub_nnf_and _ _).1, exact h},
+  {simp, right, right, apply (mem_sub_nnf_and _ _).2, exact h}}
+end
+| (box φ₁) h   := 
+begin
+simp at h,
+{split,
+ {simp, right, apply (mem_sub_nnf_and _ _).1, exact h},
+ {simp, right, apply (mem_sub_nnf_and _ _).2, exact h}}
+end
+| (dia φ₁) h   := 
+begin
+simp at h,
+{split,
+ {simp, right, apply (mem_sub_nnf_and _ _).1, exact h},
+ {simp, right, apply (mem_sub_nnf_and _ _).2, exact h}}
+end
+
+theorem mem_sub_nnf_or {φ ψ : nnf} : Π γ : nnf, or φ ψ ∈ sub_nnf γ → φ ∈ sub_nnf γ ∧ ψ ∈ sub_nnf γ
+| (var n) h   := begin simp at h, contradiction end
+| (neg n) h   := begin simp at h, contradiction end 
+| (and φ₁ ψ₁) h := 
+begin 
+simp at h,
+cases h,
+ {split,
+  {simp, right, left, apply (mem_sub_nnf_or _ _).1, exact h},
+  {simp, right, left, apply (mem_sub_nnf_or _ _).2, exact h}},
+ {split, 
+  {simp, right, right, apply (mem_sub_nnf_or _ _).1, exact h},
+  {simp, right, right, apply (mem_sub_nnf_or _ _).2, exact h}}
+end
+| (or φ₁ ψ₁) h  := 
+begin 
+simp only [sub_nnf] at h, 
+cases h, 
+{injection h with eq₁ eq₂, 
+ rw eq₁, rw eq₂, 
+ simp only [sub_nnf], 
+ split, 
+ {simp, right, left, apply mem_sub_nnf_self}, 
+ {simp, right, right, apply mem_sub_nnf_self}},
+{have := (@list.mem_append _ _ _ _).1 h,  
+ cases this,
+ {split,
+  {simp, right, left, apply (mem_sub_nnf_or _ _).1, exact this},
+  {simp, right, left, apply (mem_sub_nnf_or _ _).2, exact this}},
+ {split, 
+  {simp, right, right, apply (mem_sub_nnf_or _ _).1, exact this},
+  {simp, right, right, apply (mem_sub_nnf_or _ _).2, exact this}}}
+end
+| (box φ₁) h   := 
+begin
+simp at h,
+{split,
+ {simp, right, apply (mem_sub_nnf_or _ _).1, exact h},
+ {simp, right, apply (mem_sub_nnf_or _ _).2, exact h}}
+end
+| (dia φ₁) h   := 
+begin
+simp at h,
+{split,
+ {simp, right, apply (mem_sub_nnf_or _ _).1, exact h},
+ {simp, right, apply (mem_sub_nnf_or _ _).2, exact h}}
+end
+
+theorem mem_sub_nnf_box {φ : nnf} : Π γ : nnf, box φ ∈ sub_nnf γ → φ ∈ sub_nnf γ
+| (var n) h   := begin simp at h, contradiction end
+| (neg n) h   := begin simp at h, contradiction end 
+| (and φ₁ ψ₁) h := 
+begin 
+simp at h, 
+cases h, 
+{simp, right, left, apply mem_sub_nnf_box, exact h},
+{simp, right, right, apply mem_sub_nnf_box, exact h}
+end
+| (or φ₁ ψ₁) h  := 
+begin 
+simp at h,
+cases h, 
+{simp, right, left, apply mem_sub_nnf_box, exact h},
+{simp, right, right, apply mem_sub_nnf_box, exact h}
+end
+| (box φ₁) h   := 
+begin
+simp at h,
+cases h, 
+{rw h, simp, right, apply mem_sub_nnf_self},
+{simp, right, apply mem_sub_nnf_box, exact h}
+end
+| (dia φ₁) h   := 
+begin
+simp at h,
+simp, right, apply mem_sub_nnf_box, exact h
+end
+
+theorem mem_sub_nnf_dia {φ : nnf} : Π γ : nnf, dia φ ∈ sub_nnf γ → φ ∈ sub_nnf γ
+| (var n) h   := begin simp at h, contradiction end
+| (neg n) h   := begin simp at h, contradiction end 
+| (and φ₁ ψ₁) h := 
+begin 
+simp at h, 
+cases h, 
+{simp, right, left, apply mem_sub_nnf_dia, exact h},
+{simp, right, right, apply mem_sub_nnf_dia, exact h}
+end
+| (or φ₁ ψ₁) h  := 
+begin 
+simp at h,
+cases h, 
+{simp, right, left, apply mem_sub_nnf_dia, exact h},
+{simp, right, right, apply mem_sub_nnf_dia, exact h}
+end
+| (box φ₁) h   := 
+begin
+simp at h,
+simp, right, apply mem_sub_nnf_dia, exact h
+end
+| (dia φ₁) h   := 
+begin
+simp at h,
+cases h, 
+{rw h, simp, right, apply mem_sub_nnf_self},
+{simp, right, apply mem_sub_nnf_dia, exact h}
+end
+
+@[simp] def nnf.closure : list nnf → list nnf
+| [] := []
+| (hd::tl) := sub_nnf hd ++ nnf.closure tl
+
+theorem mem_closure_self : Π Γ : list nnf, Γ ⊆ nnf.closure Γ
+| [] := λ x h, absurd h $ list.not_mem_nil _
+| (hd::tl) := 
+begin 
+  intros x hx, cases hx, 
+  {rw hx, simp, left, apply mem_sub_nnf_self},
+  {simp, right, apply mem_closure_self, exact hx} 
+end
+
+theorem mem_closure_and {φ ψ : nnf} : Π Γ : list nnf, and φ ψ ∈ nnf.closure Γ → φ ∈ nnf.closure Γ ∧ ψ ∈ nnf.closure Γ
+| [] h := absurd h $ list.not_mem_nil _
+| (hd::tl) h := 
+begin
+simp at h,
+cases h,
+{split,
+ {simp, left, apply (mem_sub_nnf_and hd _).1, swap, exact h},
+ {simp, left, apply (mem_sub_nnf_and hd _).2, swap, exact h}},
+{split,
+ {simp, right, apply (mem_closure_and _ _).1, exact h},
+ {simp, right, apply (mem_closure_and _ _).2, exact h} }
+end
+
+theorem mem_closure_or {φ ψ : nnf} : Π Γ : list nnf, or φ ψ ∈ nnf.closure Γ → φ ∈ nnf.closure Γ ∧ ψ ∈ nnf.closure Γ
+| [] h := absurd h $ list.not_mem_nil _
+| (hd::tl) h := 
+begin
+simp at h,
+cases h,
+{split,
+ {simp, left, apply (mem_sub_nnf_or hd _).1, swap, exact h},
+ {simp, left, apply (mem_sub_nnf_or hd _).2, swap, exact h}},
+{split,
+ {simp, right, apply (mem_closure_or _ _).1, exact h},
+ {simp, right, apply (mem_closure_or _ _).2, exact h} }
+end
+
+theorem mem_closure_box {φ : nnf} : Π Γ : list nnf, box φ ∈ nnf.closure Γ → φ ∈ nnf.closure Γ
+| [] h := absurd h $ list.not_mem_nil _
+| (hd::tl) h := 
+begin
+simp at h,
+cases h,
+{simp, left, apply mem_sub_nnf_box _ h},
+{simp, right, apply mem_closure_box _ h}
+end
+
+theorem mem_closure_dia {φ : nnf} : Π Γ : list nnf, dia φ ∈ nnf.closure Γ → φ ∈ nnf.closure Γ
+| [] h := absurd h $ list.not_mem_nil _
+| (hd::tl) h := 
+begin
+simp at h,
+cases h,
+{simp, left, apply mem_sub_nnf_dia _ h},
+{simp, right, apply mem_closure_dia _ h}
+end
+
+@[simp] def filter_undia (l : list nnf) : list nnf → list nnf
+| [] := []
+| (dia φ::tl) := if φ ∈ l then filter_undia tl else φ :: filter_undia tl
+| (e::tl) := filter_undia tl
+
+theorem mem_filter_undia_left : Π l Γ φ (h₁ : dia φ ∈ Γ) (h₂ : φ ∉ l),
+φ ∈ filter_undia l Γ
+| l [] φ h₁ h₂ := absurd h₁ $ list.not_mem_nil _
+| l (hd :: tl) φ h₁ h₂ := 
+begin
+  cases h : hd,
+  case nnf.dia : ψ 
+  {rw h at h₁, simp, 
+   by_cases hc : ψ ∈ l,
+   {rw if_pos, apply mem_filter_undia_left, cases h₁, {injection h₁ with h₁', rw ←h₁' at hc, contradiction}, {exact h₁}, repeat {assumption}},
+   {rw if_neg, cases h₁, {injection h₁ with h₁', rw h₁', simp}, {right, apply mem_filter_undia_left, exact h₁, exact h₂}, exact hc}},
+  all_goals 
+  {simp, rw h at h₁, cases h₁, contradiction, apply mem_filter_undia_left, repeat {assumption}}
+end
+
+theorem mem_filter_dia_right_aux : Π l Γ φ, φ ∈ filter_undia l Γ → dia φ ∈ Γ 
+| l [] φ h := absurd h $ list.not_mem_nil _
+| l (hd :: tl) φ h := 
+begin
+cases h₁ : hd,
+case nnf.dia : ψ 
+{rw h₁ at h, dsimp at h, 
+ by_cases hc : ψ ∈ l, 
+ {rw if_pos at h, have := mem_filter_dia_right_aux l tl φ h, right, exact this, exact hc},
+ {rw if_neg at h, cases h, {rw h, simp}, {have := mem_filter_dia_right_aux l tl φ h, right, exact this}, exact hc}},
+all_goals 
+{rw h₁ at h, simp at h, right, apply mem_filter_dia_right_aux, exact h}
+end
+
+theorem mem_filter_dia_right : Π l Γ φ (h₂ : φ ∈ filter_undia l Γ), φ ∉ l
+| l [] φ h := absurd h $ list.not_mem_nil _
+| l (hd :: tl) φ h := 
+begin 
+cases h₁ : hd,
+case nnf.dia : ψ 
+{rw h₁ at h, dsimp at h, 
+ by_cases hc : ψ ∈ l, 
+ {rw if_pos at h, have := mem_filter_dia_right l tl φ h, exact this, exact hc},
+ {rw if_neg at h, cases h, {rw h, exact hc}, {have := mem_filter_dia_right l tl φ h, exact this}, exact hc}},
+all_goals 
+{rw h₁ at h, simp at h, apply mem_filter_dia_right, exact h}
+end
+
+structure hintikka (Γ : list nnf) : Prop :=
+(hno_contra : ∀ {n}, var n ∈ Γ → neg n ∉ Γ)
+(hand_left : ∀ {φ ψ}, nnf.and φ ψ ∈ Γ → φ ∈ Γ)
+(hand_right : ∀ {φ ψ}, nnf.and φ ψ ∈ Γ → ψ ∈ Γ)
+(hor : ∀ {φ ψ}, nnf.or φ ψ ∈ Γ → φ ∈ Γ ∨ ψ ∈ Γ)
+(hbox : ∀ {φ}, nnf.box φ ∈ Γ → φ ∈ Γ)
